Ghost task queue proven!

share/steel/examples/pulse/parallel/GhostTaskQueue.fst
@@ -157,20 +157,23 @@ Lemma (requires ~(get_actual_queue l == []))
 // maybe with 2/3 + 2/3 permissions
 // do I need an id (with distinctness) to compare two tasks?
 // If equality does not work, can add indices, with a uniqueness invariant...
+let task_in_queue_not_empty t pos l:
+  Lemma (requires task_in_queue t pos l)
+        (ensures L.length l >= 1)
+= ()
+
 let rec close_task #a
     //(eq: (x:a -> y:a -> b:bool{b <==> x == y }))
     (t: a)
     (pos: nat)
-    (l: mono_list a{task_in_queue t pos l}):
+    (l: mono_list a{task_in_queue t pos l /\ L.length l >= 1}):
     (s:task_status{L.memP (t, s) l} & r:mono_list a{
         s == Ongoing ==> (
             get_actual_queue r == get_actual_queue l /\
             count_ongoing r == count_ongoing l - 1)})
-= match l with
-| (t', s)::q -> 
-//if eq t t'
+= let (t', s)::q = l in
 if pos + 1 = L.length l
-  then (| s, (t', Done)::q |)
+  then (| s, (t', Done)::q |) // if s is not Ongoing, then we have too much permission
   else let (| s', q' |) = close_task t pos q in (| s', (t', s)::q' |)
 
 let rec close_task_preserves_order_aux #a
@@ -263,14 +266,35 @@ let task_elem: Type u#1 = (
 
 let task_plus: Type u#1 = task_with_status task_elem
 
+let mono_list_task_plus: Type u#1 = mono_list task_elem
+
+let certificate (r:ghost_mono_ref task_elem) (t: task_elem) (pos: nat)
+= M.witnessed r (task_in_queue t pos)
+
+// can witness that task is in queue
+let get_certificate (t: task_elem) (pos: nat)
+            (r:ghost_mono_ref task_elem)
+            //(fact:stable_property p)
+            (l:erased mono_list_task_plus)
+            (_:squash (task_in_queue t pos l))
+  : //TODO: SteelAtomicUT
+  stt_ghost (certificate r t pos)
+            emp_inames
+                  (pts_to_ghost_queue r l)
+                  (fun _ -> pts_to_ghost_queue r l)
+= witness r l _
+
+let pts_to_Some (t: task_elem & task_status): vprop
+= (exists_ (fun v -> pts_to (t._1._2) #three_quart v ** pure (Some? v)))
+
+
 // in NewDomains, g is ._3 and f is ._1
 let task_res_own (t: task_plus): vprop
 = match t._2 with
 | Todo -> pts_to (t._1._2) #three_quart None
 | Ongoing -> emp // in this case, the worker has the half permission
-| Done -> (exists_ (fun v -> pts_to (t._1._2) #three_quart v ** pure (Some? v)))
+| Done -> pts_to_Some t  //(exists_ (fun v -> pts_to (t._1._2) #three_quart v ** pure (Some? v)))
 
-let mono_list_task_plus: Type u#1 = mono_list task_elem
   
 let rec tasks_res_own (l: mono_list_task_plus): vprop
 =  match l with
@@ -278,6 +302,7 @@ let rec tasks_res_own (l: mono_list_task_plus): vprop
   | tl::ql -> task_res_own tl ** tasks_res_own ql
 
 ```pulse
+ghost
 fn fold_done_task (t: task_elem) (l:mono_list_task_plus)
   requires pts_to t._2 #three_quart None ** tasks_res_own l
   ensures tasks_res_own (enqueue_todo l t)._1
@@ -290,6 +315,460 @@ fn fold_done_task (t: task_elem) (l:mono_list_task_plus)
   ()
 }
 ```
+
+let small_inv (r: ghost_mono_ref task_elem) (q: list task_elem) (c: int): vprop 
+= exists_ (fun l -> pts_to_ghost_queue r l **
+  tasks_res_own l **
+  pure (count_ongoing l = c /\ get_actual_queue l == q)
+)
+
+#push-options "--print_universes --print_implicits"
+
+// 1: Enqueue
+```pulse
+ghost
+fn spawn_task_ghost
+(r: ghost_mono_ref task_elem)
+(q: list task_elem) (c: int) (t: task_elem)
+  requires small_inv r q c ** pts_to t._2 #three_quart None 
+  returns w: (pos:nat & certificate r t pos)
+  ensures small_inv r (t::q) c
+{
+  unfold (small_inv r q c);
+  with vl. assert (pts_to_ghost_queue r vl);
+  assert (tasks_res_own vl);
+  assert (pure (count_ongoing vl = c /\ get_actual_queue vl == q));
+  let p = enqueue_todo #task_elem vl t;
+  let pos = p._2;
+  assert (pure (task_in_queue t pos p._1));
+  write_ghost_queue #task_elem #vl r p._1;
+  assert (pts_to_ghost_queue r p._1);
+  let w: certificate r t pos = get_certificate t pos r p._1 _;
+  fold_done_task t vl;
+  fold (small_inv r (t::q) c);
+  let res = (| pos, w |);
+  res
+}
+```
+
+let rec vprop_equiv_test
+  (l: mono_list_task_plus{~(get_actual_queue l == [])})
+: vprop_equiv (tasks_res_own l)
+  (pts_to (pop_todo_task l)._1._2 #three_quart None
+  ** tasks_res_own (pop_todo_task l)._2)
+= match l with
+| (t, Todo)::q ->
+let p1: vprop_equiv (tasks_res_own l) 
+  (pts_to (pop_todo_task l)._1._2 #three_quart None ** tasks_res_own q) = vprop_equiv_refl _ in
+let p2: vprop_equiv (tasks_res_own q) (emp ** tasks_res_own q) = 
+  vprop_equiv_sym _ _ (vprop_equiv_unit _)
+ in
+let p3: vprop_equiv (emp ** tasks_res_own q) (tasks_res_own (pop_todo_task l)._2) = vprop_equiv_refl _ in
+let p4: vprop_equiv (tasks_res_own q) (tasks_res_own (pop_todo_task l)._2) = vprop_equiv_trans _ _ _ p2 p3 in
+let p5 = vprop_equiv_cong _ _ _ _ (vprop_equiv_refl (pts_to (pop_todo_task l)._1._2 #three_quart None)) p4 in
+vprop_equiv_trans _ _ _ p1 p5
+| t::q -> 
+let p1 = tasks_res_own l in
+let p2 = task_res_own t in
+let p3 = tasks_res_own q in
+let p4 = pts_to (pop_todo_task q)._1._2 #three_quart None in
+let p5 = tasks_res_own (pop_todo_task q)._2 in
+let p6 = tasks_res_own (pop_todo_task l)._2 in
+let e2: vprop_equiv p3 (p4 ** p5) = vprop_equiv_test q in
+let e3: vprop_equiv p1 (p2 ** (p4 ** p5)) = vprop_equiv_cong p2 p3 p2 (p4 ** p5) (vprop_equiv_refl _) e2 in
+let e4: vprop_equiv (p2 ** (p4 ** p5)) ((p2 ** p4) ** p5) = vprop_equiv_sym _ _ (vprop_equiv_assoc _ _ _) in
+let e5: vprop_equiv ((p2 ** p4) ** p5) ((p4 ** p2) ** p5) = vprop_equiv_cong (p2 ** p4) p5 (p4 ** p2) p5
+  (vprop_equiv_comm _ _) (vprop_equiv_refl _) in
+let e6: vprop_equiv ((p4 ** p2) ** p5) (p4 ** (p2 ** p5)) = vprop_equiv_assoc _ _ _ in
+let e7: vprop_equiv (p2 ** (p4 ** p5)) (p4 ** (p2 ** p5)) = vprop_equiv_trans _ _ _ e4 (vprop_equiv_trans _ _ _ e5 e6)
+in vprop_equiv_trans _ _ _ e3 e7
+
+let get_permission_from_todo
+  (l: mono_list_task_plus{~(get_actual_queue l == [])})
+: stt_ghost unit emp_inames
+(tasks_res_own l)
+  (fun _ -> pts_to (pop_todo_task l)._1._2 #three_quart None ** tasks_res_own (pop_todo_task l)._2)
+= rewrite _ _ (vprop_equiv_test l)
+
+// 2: Pop
+```pulse
+ghost
+fn pop_task_ghost
+(r: ghost_mono_ref task_elem)
+(t: task_elem)
+(q: list task_elem) (c: int) (t: task_elem)
+  requires small_inv r (t::q) c
+  ensures small_inv r q (c + 1) ** pts_to t._2 #three_quart None 
+{
+  unfold (small_inv r (t::q) c);
+  with l. assert (pts_to_ghost_queue r l);
+  assert (tasks_res_own l);
+  assert (pure (count_ongoing l = c /\ get_actual_queue l == t::q));
+  let p = pop_todo_task #task_elem l;
+  let order_is_preserved = pop_preserves_order #task_elem l;
+  write_ghost_queue #task_elem #l r p._2;
+  assert (pts_to_ghost_queue r p._2);
+  assert (pure (p._1 == t));
+  get_permission_from_todo l;
+  fold (small_inv r q (c + 1));
+  rewrite (pts_to (pop_todo_task l)._1._2 #three_quart None)
+    as (pts_to t._2 #three_quart None);
+  ()
+}
+```
+
+// To prove
+assume val equiv_not_aliases (#a: Type) (r1 r2: ref a) (v1 v2: a):
+vprop_equiv
+  (pts_to r1 #three_quart v1 ** pts_to r2 #three_quart v2)
+  (pts_to r1 #three_quart v1 ** pts_to r2 #three_quart v2 ** pure (~(r1 == r2)))
+
+let derive_false_from_too_much_permission (#a: Type) (r: ref a) (v1 v2: a):
+stt_ghost unit emp_inames (pts_to r #three_quart v1 ** pts_to r #three_quart v2)
+(fun () ->
+pts_to r #three_quart v1 ** pts_to r #three_quart v2 **
+pure (~(r == r)))
+= rewrite _ _ (equiv_not_aliases r r v1 v2)
+
+
+// TODO: Do this vprop_equiv
+
+(*
+let rec vprop_equiv_test
+  (l: mono_list_task_plus{~(get_actual_queue l == [])})
+: vprop_equiv (tasks_res_own l)
+  (pts_to (pop_todo_task l)._1._2 #three_quart None
+  ** tasks_res_own (pop_todo_task l)._2)
+= match l with
+| (t, Todo)::q ->
+let p1: vprop_equiv (tasks_res_own l) 
+  (pts_to (pop_todo_task l)._1._2 #three_quart None ** tasks_res_own q) = vprop_equiv_refl _ in
+let p2: vprop_equiv (tasks_res_own q) (emp ** tasks_res_own q) = 
+  vprop_equiv_sym _ _ (vprop_equiv_unit _)
+ in
+let p3: vprop_equiv (emp ** tasks_res_own q) (tasks_res_own (pop_todo_task l)._2) = vprop_equiv_refl _ in
+let p4: vprop_equiv (tasks_res_own q) (tasks_res_own (pop_todo_task l)._2) = vprop_equiv_trans _ _ _ p2 p3 in
+let p5 = vprop_equiv_cong _ _ _ _ (vprop_equiv_refl (pts_to (pop_todo_task l)._1._2 #three_quart None)) p4 in
+vprop_equiv_trans _ _ _ p1 p5
+| t::q -> 
+*)
+
+(*
+let rec put_back_permission_equiv
+  (t: task_elem)
+  (pos: nat)
+  (l: mono_list_task_plus{task_in_queue t pos l})
+  (x: t._1)
+: vprop_equiv 
+  (tasks_res_own l ** pts_to t._2 #three_quart (Some x))
+  (tasks_res_own (close_task t pos l)._2 **
+  pure (Ongoing? (close_task t pos l)._1))
+= match l with
+| (t', s)::q -> 
+if pos + 1 = L.length l
+  then admit() //(| s, (t', Done)::q |)
+  else let (| s', q' |) = close_task t pos q in
+  assert (close_task t pos l == (| s', (t', s)::q' |));
+  admit() // (| s', (t', s)::q' |)
+  *)
+
+  (*
+   match l with
+| (t', s)::q -> 
+//if eq t t'
+if pos + 1 = L.length l
+  then (| s, (t', Done)::q |) // if s is not Ongoing, then we have too much permission
+  else let (| s', q' |) = close_task t pos q in (| s', (t', s)::q' |)
+  *)
+
+(*
+= match l with
+| (t', s)::q -> 
+//if eq t t'
+if pos + 1 = L.length l
+  then (| s, (t', Done)::q |)
+  else let (| s', q' |) = close_task t pos q in (| s', (t', s)::q' |)
+*)
+//let decompose_list (l: mono_list_task_plus{L.length l > 0}):
+//  Lemma (L.hd l == ((L.hd l)._1, (L.hd l)._2))
+//  = ()
+let rec close_task_bis #a
+    //(eq: (x:a -> y:a -> b:bool{b <==> x == y }))
+    (t: a)
+    (pos: nat)
+    (l: mono_list a{task_in_queue t pos l /\ L.length l >= 1}):
+  mono_list a
+  (*
+    (s:task_status{L.memP (t, s) l} & r:
+    mono_list a{
+        s == Ongoing ==> (
+            get_actual_queue r == get_actual_queue l /\
+            count_ongoing r == count_ongoing l - 1)})
+*)
+= let (t', s)::q = l in
+if pos + 1 = L.length l
+  then (t', Done)::q // if s is not Ongoing, then we have too much permission
+  else (t', s)::(close_task_bis t pos q)
+
+let rec close_task_bis_preserves_order_aux #a
+    (t: a)
+    (pos: nat)
+    (l: mono_list a{task_in_queue t pos l}):
+    Lemma (is_same_mono_list l (close_task_bis t pos l) )
+= match l with
+| (t', s)::q -> if pos + 1 = L.length l then is_mono_suffix_refl q
+else let q' = close_task_bis t pos q in close_task_bis_preserves_order_aux t pos q
+
+
+
+let close_task_bis_preserves_order #a
+    (t: a)
+    (pos: nat)
+    (l: mono_list a{task_in_queue t pos l}):
+    Lemma (is_mono_suffix l (close_task_bis t pos l) )
+= close_task_bis_preserves_order_aux t pos l; from_same_to_suffix l (close_task_bis t pos l)
+
+
+
+// waiting to have recursion in Pulse
+assume val put_back_permission_cb
+  (t: task_elem)
+  (pos: nat)
+  (l: (l:mono_list_task_plus{task_in_queue t pos l /\ L.length l >= 1}))
+  (x: t._1)
+:
+stt_ghost unit emp_inames
+(tasks_res_own l ** pts_to t._2 #three_quart (Some x))
+(fun () -> tasks_res_own (close_task_bis t pos l) ** pure (
+ get_actual_queue (close_task_bis t pos l) == get_actual_queue l
+  /\ count_ongoing (close_task_bis t pos l) + 1 == count_ongoing l))
+
+
+```pulse
+ghost
+fn derive_status_ongoing (h: (task_elem & task_status)) (x: h._1._1)
+  requires task_res_own h ** (pts_to (h._1._2) #three_quart (Some x))
+  ensures task_res_own h ** (pts_to (h._1._2) #three_quart (Some x)) ** pure (h._2 = Ongoing)
+{
+  if (snd h = Todo) {
+    rewrite (task_res_own h) as (pts_to (h._1._2) #three_quart None);
+    derive_false_from_too_much_permission h._1._2 None (Some x);
+    assert (pure (h._2 = Ongoing));
+    rewrite (pts_to (h._1._2) #three_quart None) as (task_res_own h);
+    ()
+  }
+  else {
+    if (snd h = Done) {
+      rewrite (task_res_own h) as (pts_to_Some h);
+      unfold (pts_to_Some h);
+      assert (exists_ (fun v -> pts_to (h._1._2) #three_quart v ** pure (Some? v)));
+      with v. assert (pts_to (h._1._2) #three_quart v ** pure (Some? v));
+      ////with v. assert (pts_to h._1._2 v);
+      derive_false_from_too_much_permission h._1._2 v (Some x);
+      fold (pts_to_Some h);
+      rewrite (pts_to_Some h) as (task_res_own h);
+      ()
+    }
+    else {
+      ()
+    }
+  }
+}
+```
+
+```pulse
+ghost
+fn fold_task_done (h:(task_elem & task_status))
+  requires pts_to h._1._2 #three_quart (Some x) ** pure (h._2 = Done)
+  ensures task_res_own h
+{
+  assert (pts_to h._1._2 #three_quart (Some x) ** pure (Some? (Some x)));
+  intro_exists (fun v -> pts_to h._1._2 #three_quart v ** pure (Some? v)) (Some x);
+  rewrite (exists_ (fun v -> pts_to h._1._2 #three_quart v ** pure (Some? v))) as (pts_to_Some h);
+  rewrite (pts_to_Some h) as (task_res_own h);
+  ()
+}
+```
+(*
+    let h' = (h._1, Done);
+    rewrite (pts_to (h._1._2) #three_quart (Some x)) as (pts_to h'._1._2 #three_quart (Some x));
+    //rewrite (pts_to h'._1._2 #three_quart (Some x)) as
+     // (exists v. pts_to (h'._1._2) #three_quart v ** pure (Some? v));
+
+    rewrite (pts_to (h._1._2) #three_quart (Some x))
+    as `@(match h'._2 with
+      | Todo -> pts_to (h'._1._2) #three_quart None
+      | Ongoing -> emp
+      | Done -> (exists_ (fun v -> pts_to (h'._1._2) #three_quart v ** pure (Some? v))));
+    *)
+
+```pulse
+ghost
+fn fold_tasks_res_own (h: (task_elem & task_status)) (q: mono_list_task_plus)
+//: stt_ghost unit emp_inames
+requires task_res_own h ** tasks_res_own q
+ensures tasks_res_own (h::q)
+{
+  rewrite (task_res_own h ** tasks_res_own q) as (tasks_res_own (h::q));
+  ()
+}
+```
+//= rewrite ()
+
+```pulse
+ghost
+fn put_back_permission
+  (t: task_elem)
+  (pos: nat)
+  (l: (l:mono_list_task_plus{task_in_queue t pos l /\ L.length l >= 1}))
+  (x: t._1)
+requires tasks_res_own l ** pts_to t._2 #three_quart (Some x)
+ensures tasks_res_own (close_task_bis t pos l) ** pure (
+ get_actual_queue (close_task_bis t pos l) == get_actual_queue l
+  /\ count_ongoing (close_task_bis t pos l) + 1 == count_ongoing l)
+{
+  let h = L.hd l;
+  let q = L.tl l;
+
+  unfold (tasks_res_own l);
+  rewrite `@(
+  match l with
+    | [] -> emp
+    | tl::ql -> task_res_own tl ** tasks_res_own ql)
+  as (task_res_own h ** tasks_res_own q);
+  assert (pts_to t._2 #three_quart (Some x));
+  assert (task_res_own h ** tasks_res_own q);
+
+  if (pos + 1 = L.length l)
+  {
+    assert (task_res_own h);
+    rewrite (pts_to (t._2) #three_quart (Some x)) as (pts_to (h._1._2) #three_quart (Some x));
+    derive_status_ongoing h x;
+    assert (pure (snd h = Ongoing));
+    assert (pts_to (h._1._2) #three_quart (Some x));
+
+    unfold (task_res_own h); // not needed, can be dropped
+    rewrite `@(match h._2 with
+      | Todo -> pts_to (h._1._2) #three_quart None
+      | Ongoing -> emp
+      | Done -> (exists_ (fun v -> pts_to (h._1._2) #three_quart v ** pure (Some? v))))
+    as (emp);
+
+    let h' = (h._1, Done);
+    rewrite (pts_to (h._1._2) #three_quart (Some x)) as (pts_to h'._1._2 #three_quart (Some x));
+    fold_task_done h';
+    fold_tasks_res_own h' q;
+    ()
+  }
+  else {
+    put_back_permission_cb t pos q x;
+    assert (tasks_res_own (close_task_bis t pos q));
+    assert (pure (get_actual_queue (close_task_bis t pos q) == get_actual_queue q));
+    assert (pure (get_actual_queue (close_task_bis t pos l) == get_actual_queue l));
+    assert (pure (count_ongoing (close_task_bis t pos q) + 1 == count_ongoing q));
+    assert (pure (count_ongoing (close_task_bis t pos l) + 1 == count_ongoing l));
+
+    rewrite (task_res_own h ** tasks_res_own (close_task_bis t pos q)) as
+    `@(
+    match (close_task_bis t pos l) with
+      | [] -> emp
+      | tl::ql -> task_res_own tl ** tasks_res_own ql);
+    fold (tasks_res_own (close_task_bis t pos l));
+    ()
+  }
+}
+```
+
+(*
+  //Ongoing? (close_task t pos l)._1)
+{
+  assert (pure (L.length l > 0));
+  (*
+= let (t', s)::q = l in
+if pos + 1 = L.length l
+  then (| s, (t', Done)::q |) // if s is not Ongoing, then we have too much permission
+  else let (| s', q' |) = close_task t pos q in (| s', (t', s)::q' |)
+  *)
+  //let h: ((task_elem u#1) & task_status) = L.hd l;
+  let h: (task_with_status u#1 task_elem) = L.hd l;
+// type task_with_status (a: Type) = a & task_status
+  let t': task_elem = fst h;
+  let s: task_status = snd h;
+  //assert (pure (h == (t', s)));
+  assert (pure (fst h == t'));
+  assert (pure (snd h == s));
+  assert (pure (eq2 h (Mktuple2 #task_elem #task_status t' s)));
+
+  let q = L.tl l;
+  //assert (pure (l == (t', s)::q));
+  //assert (pure (h == (t', s)));
+  //let proof = decompose_list l;
+  //rewrite emp as (pure (L.hd l == (t', s)));
+  //assert (pure (L.hd l == (t', s))); // why needed?
+  assert (pure (l == (L.hd l)::q));
+  //assert (pure (l == (t', s)::q));
+  //inhale (pure (L.hd l == (t', s))); // why needed?
+  //rewrite emp as (pure (l == ((t', s)::q))); // unclear...
+  //assert (pure (l == ((t', s)::q))); // unclear...
+  //inhale (pure ( l == (t', s)::q ));
+  //inhale (pure ( l == (t', s)::q ));
+  if (pos + 1 = L.length l)
+  {
+    let pair: (tuple2 u#1 u#0 task_elem task_status) = Mktuple2 #task_elem #task_status t' Done;
+    let pairq = Cons #(tuple2 u#1 u#0 task_elem task_status) pair q;
+    let dtup = Mkdtuple2 #task_status #_ s pairq;
+    assert (pure (close_task t pos l == dtup));
+    // task must be t
+    // status can be only Ongoing, otherwise we derive a contradiction
+    admit()
+  }
+  else
+  {
+    // recursive call
+    admit()
+  }
+  (*
+= match l with
+| (t', s)::q -> 
+if pos + 1 = L.length l
+  then admit() //(| s, (t', Done)::q |)
+  else let (| s', q' |) = close_task t pos q in admit() // (| s', (t', s)::q' |)
+  *)
+}
+```
+*)
+
+
+
+
+// 3: conclude the task
+```pulse
+ghost
+fn conclude_task_ghost
+(t: task_elem)
+(pos: nat)
+(r: ghost_mono_ref task_elem)
+(q: list task_elem) (c: int)
+(x: t._1)
+(w: certificate r t pos)
+  requires small_inv r q c ** pts_to t._2 #three_quart (Some x)
+  ensures small_inv r q (c - 1) 
+{
+  unfold (small_inv r q c);
+  with l. assert (pts_to_ghost_queue r l);
+  assert (tasks_res_own l);
+  assert (pure (count_ongoing l = c /\ get_actual_queue l == q));
+  let proof = recall #task_elem #t #pos r l w;
+  let p = close_task_bis t pos l;
+  let order_is_preserved = close_task_bis_preserves_order #task_elem t pos l;
+  write_ghost_queue #task_elem #l r p;
+  put_back_permission t pos l x;
+  assert (tasks_res_own (close_task_bis t pos l));
+  fold (small_inv r q (c - 1));
+  ()
+}
+```
+
 
 (*
 Need:
